theories/Spilling/RepairSpillSound.v
@@ -40,10 +40,29 @@ Proof.
   - destruct a,p. rename s0 into Sp. rename s1 into L. rename a0 into Rlv.
     set (L' := pick_load k R M Sp L (Exp.freeVars e)) in *.
     set (K' := pick_kill k R L' (Exp.freeVars e) Rlv) in *.
-    set (Kx' := pick_killx k x (R \ K' ∪ L') Rlv) in *.
+    set (Kx' := pick_killx k (R \ K' ∪ L') Rlv) in *.
     set (Sp':= (getAnn al ∩ (K' ∪ Kx') \ M ∪ (Sp ∩ R))) in *.
     assert (Sp ∩ R ⊆ Sp') as Spincl.
     { subst Sp'. clear; cset_tac. }
+    assert (K' ⊆ R) as KReq.
+    { subst K'. rewrite pick_kill_incl. clear; cset_tac. }
+    assert (disj (R \ K') L') as RKLdisj.
+    { subst K'. rewrite <-incl_pick_kill. clear. cset_tac. }
+    assert (cardinal (R \ K' ∪ L') <= k) as card_RKL.
+    {
+      rewrite union_cardinal; [|clear - RKLdisj;intros;intro N;cset_tac].
+      rewrite cardinal_difference'; eauto.
+      rewrite <-Nat.add_sub_swap; [|rewrite subset_cardinal; eauto].
+      apply Nat.le_sub_le_add_r.
+      subst K'. rewrite <-pick_kill_card; [omega|].
+      subst L'. rewrite pick_load_card; eauto.
+      assert (forall n1 n2 n3 : nat, n1 <= n3 -> n3 <= n2 -> n1 + (n2 - n3) <= n2) as nateq.
+      { clear. intros. omega. }
+      apply nateq; eauto.
+      * apply subset_cardinal;eauto. rewrite <-incl_pick_load; eauto.
+        clear;cset_tac.
+      * rewrite subset_cardinal; eauto. clear; cset_tac.
+    }
     econstructor; eauto; cbn in *.
     + subst Sp'. subst K'. rewrite pick_kill_incl. setoid_rewrite meet_in_left at 2.
       subst Kx'. rewrite pick_killx_incl.
@@ -64,11 +83,35 @@ Proof.
       setoid_rewrite union_comm at 2. rewrite <-minus_union, minus_minus.
       rewrite incl_minus_union; [|clear;cset_tac].
       subst L'. rewrite <-incl_pick_load. clear; cset_tac.
-    + assert (K' ⊆ R) as KReq.
-      { subst K'. rewrite pick_kill_incl. clear; cset_tac. }
-      assert (disj (R \ K') L') as RKLdisj.
-      { subst K'. rewrite <-incl_pick_kill. clear. cset_tac. }
-      rewrite union_cardinal; [|clear - RKLdisj;intros;intro N;cset_tac].
+    + decide (x ∈ (R \ K' ∪ L') \ Kx').
+      * rewrite add_cardinal_1; eauto. rewrite cardinal_difference'; [| apply pick_killx_incl].
+        apply Nat.le_sub_le_add_r. rewrite card_RKL. omega.
+      * rewrite add_cardinal_2; eauto. rewrite cardinal_difference'; [| apply pick_killx_incl].
+        rewrite minus_Sn_m. Focus 2. apply subset_cardinal. subst Kx'. apply pick_killx_incl.
+        apply Nat.le_sub_le_add_r. subst Kx'. rewrite <-pick_killx_card.
+        -- omega.
+        -- setoid_rewrite union_comm at 2. rewrite <-set_decomp. omega.
+  - destruct a. destruct p as (Sp, L). cbn in *. rename sa0 into rlv1. rename ta0 into rlv2.
+    set (L' := pick_load k R M Sp L (Op.freeVars e)) in *.
+    set (K' := pick_kill k R L' (Op.freeVars e) (getAnn rlv1 ∪ getAnn rlv2)) in *.
+    set (Sp':= ((getAnn al1 ∪ getAnn al2) ∩ K' \ M) ∪ (Sp ∩ R)) in *.
+    assert (Sp ∩ R ⊆ Sp') as Spincl.
+    { subst Sp'. clear; cset_tac. }
+    assert (K' ⊆ R) as KReq.
+    { subst K'. rewrite pick_kill_incl. clear; cset_tac. }
+    assert (disj (R \ K') L') as RKLdisj.
+    { subst K'. rewrite <-incl_pick_kill. clear. cset_tac. }
+    econstructor; eauto; cbn in *.    
+    + subst Sp'. subst K'. rewrite pick_kill_incl. setoid_rewrite meet_in_left at 2.
+      setoid_rewrite minus_incl at 2 3.
+      rewrite H0, H1. rewrite lv_RM. clear; cset_tac.
+    + subst L'. rewrite pick_load_incl. rewrite <-Spincl.
+      cbn in *. apply Op.freeVars_live in H. rewrite H. clear - lv_RM. cset_tac.
+    + instantiate (1:=K'). subst K'. rewrite pick_kill_incl.
+      setoid_rewrite union_comm at 2. rewrite <-minus_union, minus_minus.
+      rewrite incl_minus_union; [|clear;cset_tac].
+      subst L'. rewrite <-incl_pick_load. clear; cset_tac.
+    + rewrite union_cardinal; [|clear - RKLdisj;intros;intro N;cset_tac].
       rewrite cardinal_difference'; eauto.
       rewrite <-Nat.add_sub_swap; [|rewrite subset_cardinal; eauto].
       apply Nat.le_sub_le_add_r.
@@ -78,9 +121,37 @@ Proof.
       { clear. intros. omega. }
       apply nateq; eauto.
       * apply subset_cardinal;eauto. rewrite <-incl_pick_load; eauto.
-        admit. (*rewrite <-incl_pick_load. clear; cset_tac.*)
+        clear;cset_tac.
       * rewrite subset_cardinal; eauto. clear; cset_tac.
-    + 
-  - 
-  
-                
+    + eapply IHlvSnd1; eauto.
+      setoid_rewrite <-inter_subset_equal with (s':=getAnn al1) at 1; eauto.
+      setoid_rewrite H0 at 1. subst Sp'.
+      clear - lv_RM. cbn in *. rewrite lv_RM. rewrite union_meet_distr_r.
+      apply union_incl_split; [cset_tac|].
+      clear; cset_tac.
+    + eapply IHlvSnd2; eauto.
+      setoid_rewrite <-inter_subset_equal with (s':=getAnn al2) at 1; eauto.
+      setoid_rewrite H1 at 1. subst Sp'.
+      clear - lv_RM. cbn in *. rewrite lv_RM. rewrite union_meet_distr_r.
+      apply union_incl_split; [cset_tac|].
+      clear; cset_tac.
+  - admit.
+  - destruct a. destruct p as [Sp L]. cbn in *.
+    set (L' := pick_load k R M Sp L (Op.freeVars e)) in *.
+    econstructor; eauto.
+    + cset_tac.
+    + subst L'. rewrite pick_load_incl. 
+      apply Op.freeVars_live in H. rewrite H. clear - lv_RM. cset_tac.
+    + instantiate (1:=(R \ Op.freeVars e) ∪ (R ∩ L')). rewrite <-minus_union.
+      rewrite incl_minus_union; [|clear;cset_tac]. rewrite minus_minus.
+      subst L'. setoid_rewrite <-incl_pick_load. clear; cset_tac'.
+    + rewrite <-minus_union.
+      rewrite union_cardinal; [|clear;intros;intro N;cset_tac].
+      subst L'. rewrite pick_load_card; eauto. rewrite <-incl_pick_load.
+      rewrite minus_minus.
+      assert (forall n1 n2 n3 n4 : nat, n1 <= n3 -> n3 <= n2 -> n1 + (n2 - n3) <= n2) as nateq.
+        { clear. intros. omega. }
+        apply nateq; eauto.
+        -- apply subset_cardinal;eauto. clear; cset_tac. 
+        -- rewrite subset_cardinal;eauto. clear; cset_tac.
+  - admit.
